Extracted remove proof, added some hints to solve_typing  to help with lctx_lft_alive proofs, TODO these should probably be moved

theories/typing/lib/ghostptrtoken/ghostptrtoken_insertremove.v
@@ -1,10 +1,28 @@
 From lrust.typing Require Export type.
-From lrust.typing Require Import uniq_util typing ptr ghost.
+From lrust.typing Require Import uniq_util typing ptr logic_fn.
 From lrust.typing.lib.ghostptrtoken Require Import ghostptrtoken_basic ghostseq_basic permdata_basic.
 Set Default Proof Using "Type".
 
 Open Scope nat.
 Implicit Type 𝔄 𝔅: syn_type.
+
+Section lft_contexts_addition.
+  Context `{!typeG Σ}.
+
+  Lemma lctx_lft_alive_intersect_list αl E L:
+    (∀ α, α ∈ αl → lctx_lft_alive E L α) →
+    lctx_lft_alive E L (lft_intersect_list αl).
+  Proof.
+    rewrite -Forall_forall. intros H. induction αl; inversion_clear H. apply lctx_lft_alive_static.
+    simpl. apply lctx_lft_alive_intersect. done. apply IHαl. done.
+  Qed.
+
+  Lemma elem_of_ty_outlives_E {𝔄} ϝ x (ty: type 𝔄) : x ∈ ty_lfts ty → ϝ ⊑ₑ x ∈ ty_outlives_E ty ϝ .
+  Proof.
+    intros. rewrite elem_of_list_fmap. eexists. done.
+  Qed.
+End lft_contexts_addition.
+Global Hint Resolve lctx_lft_alive_intersect_list elem_of_ty_outlives_E: lrust_typing.
 
 Section ghostptrtoken_insertremove.
   Context `{!typeG Σ}.
@@ -30,9 +48,77 @@ Section ghostptrtoken_insertremove.
     apply not_elem_of_list_to_map_1. inversion_clear nodup. done.
   Qed.
 
+  Definition find_idx {A} P `{∀ x, Decision (P x)} : list A → nat :=
+    fix go l :=
+    match l with
+    | [] => 0
+    | x :: l => if decide (P x) then 0 else S (go l)
+    end.
+  
+
+  Lemma find_idx_alt {A} P `{∀ x, Decision (P x)} (l: list A):
+    find_idx P l = match list_find P l with | Some x => x.1 | None => length l end.
+  Proof. 
+    induction l; simpl. done. destruct (decide (P a)); simpl. done. 
+    rewrite IHl. destruct (list_find P l); done.
+  Qed.
+
+  Lemma find_idx_spec' {A} P `{∀ x, Decision (P x)} (l: list A) (i: nat):
+  find_idx P l = i ↔
+    (i = length l ∨ ∃ x, l !! i = Some x ∧ P x) ∧ ∀ j y, l !! j = Some y → j < i → ¬P y.
+  Proof.
+    rewrite find_idx_alt. remember (list_find P l) as x. symmetry in Heqx. remember Heqx as eq. clear Heqeq. destruct x as [[??]|].
+    rewrite list_find_Some in Heqx. destruct Heqx as (?&?&?). split.  move=>/=<-. split. right. exists a. done. done.
+    intros ([|[?[??]]]&?). exfalso; eapply H4. exact H0. rewrite H3. eapply lookup_lt_Some. done. done.
+    assert (list_find P l = Some (i, x)). rewrite list_find_Some. done.
+    rewrite eq in H6. injection H6. done.
+    rewrite list_find_None Forall_forall in Heqx. split. intros. split. left. done. intros. apply Heqx. eapply elem_of_list_lookup_2. done.
+    intros ([|[?[??]]]&?). done. assert (list_find P l = Some (i, x)). rewrite list_find_Some. done.
+    rewrite eq in H3. done.
+  Qed.
+
+  Lemma find_idx_spec {A} P `{∀ x, Decision (P x)} (l: list A):
+    (find_idx P l = length l ∨ ∃ x, l !! find_idx P l = Some x ∧ P x) ∧ ∀ j y, l !! j = Some y → j < find_idx P l  → ¬P y.
+  Proof.
+    remember (find_idx P l) as f. symmetry in Heqf. rewrite find_idx_spec' in Heqf. done.
+  Qed.
+
+  Lemma find_idx_Some {A} P `{∀ x, Decision (P x)} (l: list A) (x: A):
+    l !! find_idx P l = Some x → P x.
+  Proof.
+    destruct (find_idx_spec P l) as [[|[?[??]]]?].
+    rewrite H0. intros. apply lookup_lt_Some in H2. lia. 
+    rewrite H0. intros [= ->]. done.
+  Qed.
+
+  Lemma find_idx_fmap {A B} P `{∀ x, Decision (P x)} (l: list B) (f: B → A): find_idx P (f<$>l) = find_idx (P ∘ f) l.
+  Proof.
+    rewrite 2! find_idx_alt list_find_fmap. remember (list_find (P ∘ f) l) as x. destruct x. done. rewrite fmap_length. done.
+  Qed.
+
+  Lemma find_idx_delete {K A} `{EqDecision K} `{FinMap K M} (l: list (K*A)) (k: K) (a: A):
+    ((list_to_map l): M A) !! k = Some a → <[k:=a]>(list_to_map (base.delete (find_idx (λ x, x.1 = k) l) l): M A) = (list_to_map l) ∧ l !! (find_idx (λ x, x.1 = k) l) = Some (k, a).
+  Proof.
+    induction l as [|[??]]; simpl. rewrite lookup_empty. done.
+    destruct (decide (k0 = k)) as [->|?]; simpl. rewrite lookup_insert. intros [= ->]. done.
+    intros ?. rewrite lookup_insert_ne in H7; [|done]. destruct (IHl H7) as (<-&<-). rewrite -insert_commute; done.
+  Qed.
+
+  Lemma find_logic {𝔄 𝔄'} (ty: type (𝔄*𝔄')) (ty': plain_type 𝔄) `{!EqDecision 𝔄} :
+    (∀ vπ ξl, ty_proph ty vπ ξl → ∃ (x: 𝔄) (vπ': proph 𝔄'), vπ = (λ π, (x, vπ' π))) → logic_fn +[ghostseq.ghostseq_ty ty; (ty': type 𝔄)] int (λ '-[l; k], find_idx (λ (x: (𝔄*𝔄')) , x.1 = k) l).
+  Proof. intros ? (?&?&[]) ((?&?&?&->&->&?)&(?&?&->)&[]). exists [].
+    revert x1 H0. simpl. induction x0 as [|fst rest]; intros; destruct x1; inversion_clear H0. exists 0%Z. done.
+    destruct (H _ _ H1) as (fst'&?&->).  simpl. destruct (decide (fst' = x2)). exists 0%Z. done.
+    destruct (IHrest x1 H2) as (res&eq). exists (Z.succ res). fun_ext=>π/=. specialize (equal_f eq π)=>/=<-. lia.
+  Qed.
+
+
   Definition ghostptrtoken_remove {𝔄} (ty: type 𝔄) : val :=
     fn: ["t"; "ptr"] :=
+      Skip;;
       delete [ #1; "t"];;
+      (Skip;;Skip);;
+      (Skip;;Skip);;
       return: ["ptr"].
 
   (* Rust's GhostPtrToken::remove *)
@@ -40,70 +126,20 @@ Section ghostptrtoken_insertremove.
     typed_val (ghostptrtoken_remove ty) (fn<α>(∅; &uniq{α} (ghostptrtoken_ty ty), ptr) → box ty)
       (λ post '-[(al, al'); p], exists(a: 𝔄), ((list_to_gmap al) !! p = Some a) ∧ ((<[p:=a]>(list_to_gmap al') = (list_to_gmap al)) → post a)).
   Proof.
-    eapply type_fn; [apply _|]=> α ??[l[x[]]]. simpl_subst.
-    iIntros (?(lπ & pπ &[]) ?) "#LFT #TIME #PROPH #UNIQ #E Na L C /=(l & x &_) #Obs".
-    rewrite !tctx_hasty_val. iDestruct "l" as ([|dl]) "[_ l]"=>//.
-    case l as [[|l|]|]=>//. iDestruct "l" as "[(%ll & >↦l & [#LftIn uniq]) †l]".
-    case ll as [|[[|l'|]|][]]; try by iDestruct "uniq" as ">[]".
-    iDestruct "x" as ([|dx]) "[⧖x x]"=>//. case x as [[|x|]|]=>//=.
-    iDestruct "x" as "[x' †x]".
-     wp_bind (delete _). rewrite freeable_sz_full.
-    iApply ((wp_delete [ #l'])with "[↦l †l]"); [done| by iFrame|]. 
-    iNext. iIntros.
-    iDestruct "x'" as (?) "(↦x&x')".
-    iDestruct "x'" as (p) "(%pπeq& %vleq)".
-    iDestruct "uniq" as (du ξi [? Eq2]) "[Vo Bor]".
-    move: Eq2. set ξ := PrVar _ ξi=> Eq2.
-    iMod (lctx_lft_alive_tok α with "E L") as (?) "(α & L & ToL)"; [solve_typing..|].
-    iMod (bor_acc with "LFT Bor α") as "[(%&%& ⧖u & Pc & ↦token) ToBor]"; [done|].
-    wp_seq. 
-    iDestruct (uniq_agree with "Vo Pc") as %[<-<-].
-    rewrite split_mt_token.
-    iDestruct "↦token" as (aπl Eq1) "(↦l & ↦token)".
-    iCombine "⧖u ⧖x" as "#⧖". simpl.
-    iMod (proph_obs_sat with "PROPH Obs") as "%ObsSat"; [done|].
-    remember ((list_to_gmap aπl) !! p) as bπ. symmetry in Heqbπ. destruct bπ as [bπ|]; last first.
-    destruct ObsSat. rewrite (surjective_pairing_fun lπ) in H1.
-    rewrite Eq1 in H1. rewrite pπeq in H1. simpl in H1. 
-    destruct H1 as (?&Contains&?).
-    rewrite /alapply list_to_map_fmap lookup_fmap Heqbπ in Contains. done.
-    destruct (elem_of_list_to_map_2' _ _ _ Heqbπ) as (rπ&perm&reinsert).
-    iEval (rewrite perm 2! big_sepL_cons) in "↦token".
-    iDestruct "↦token" as "((↦x' & ↦) & †x' & †)".
-    destruct du; [done|].
-    iMod (uniq_update with "UNIQ Vo Pc") as "[Vo Pc]"; [done|].
-    replace (S du `max` dx) with (S (du `max` (pred dx))); [|lia].
-    iMod ("ToBor" with "[↦l ↦ † Pc]") as "[Bor α]".
-    { iNext. iExists _, _. rewrite split_mt_token. iFrame "⧖ Pc".
-      iExists _. iFrame. iSplit; [done|].
-      iApply (big_sepL_impl with "↦"). iModIntro. iIntros (?[??]?) "H".
-      iDestruct "H" as (?) "(H1&H2)". iExists _. iFrame. iApply (ty_own_depth_mono with "H2"). lia.
-    }
-    iMod ("ToL" with "α L") as "L".
-    set lπ' := λ π, ((alapply rπ π), π ξ).
-    iApply (type_type +[#l' ◁ &uniq{α} (ghostptrtoken_ty ty); #x ◁ box (box ty)] -[lπ'; bπ]
-    with "[] LFT TIME PROPH UNIQ E Na L C [-] []").
-    - iApply type_jump; [solve_typing|solve_extract|solve_typing].
-    - iSplitL "Vo Bor"; [|iSplitL; [|done]]. rewrite (tctx_hasty_val #l').
-      iExists _. iSplit; [done|]. 
-      iSplit; [done|]. fold max. iExists _, _. rewrite /uniq_body.
-      rewrite (proof_irrel (@prval_to_inh (listₛ (locₛ * 𝔄)) (fst ∘ lπ')) (@prval_to_inh (listₛ (locₛ * 𝔄)) (fst ∘ lπ))).
-      replace (fst ∘ lπ') with (alapply rπ); [|done].
-      iFrame. iPureIntro. split; [done|done].
-      rewrite (tctx_hasty_val #x). iExists _. iSplit; [done|]. rewrite vleq.
-      simpl. iFrame. iNext. iExists _. 
-      iFrame. simpl. rewrite freeable_sz_full. iFrame. 
-      iNext. iDestruct "↦x'" as (?) "(a & rest)". iExists vl0. iFrame.
-      iApply ty_own_depth_mono; [|done]. lia.
-    - iApply proph_obs_impl; [|done]=> π.
-      move: (equal_f Eq1 π) (equal_f Eq2 π)=>/=. case (lπ π)=>/= ??->-> Imp Eq.
-      destruct Imp as (xv&xeq&Imp).
-      rewrite /alapply list_to_map_fmap lookup_fmap_Some in xeq. destruct xeq as (xπ&<-&lookup_eq).
-      rewrite (equal_f pπeq)/= in lookup_eq.
-      rewrite lookup_eq in Heqbπ. injection Heqbπ as ->.
-      apply Imp. rewrite Eq.
-      rewrite /alapply 2! list_to_map_fmap -fmap_insert. f_equal.
-      rewrite (equal_f pπeq). exact.
+    intros ?. eapply type_fn; [apply _|]=> α ??[l[l2[]]]. simpl_subst. via_tr_impl.
+    iApply ghost_read_delete; [done|]. iIntros. iApply ghost_new; [solve_typing|].
+    iApply typed_body_tctx_incl. eapply tctx_incl_trans. eapply tctx_incl_tail. apply tctx_incl_swap. apply tctx_incl_swap.
+    iApply ghost_new; [solve_typing|].
+    iApply typed_body_tctx_incl. eapply tctx_incl_trans. eapply tctx_incl_tail. eapply tctx_incl_trans. apply tctx_incl_swap. eapply tctx_incl_tail. apply tctx_incl_swap.
+    eapply tctx_incl_trans. eapply (tctx_incl_frame_r +[_; _]). eapply tctx_incl_trans. eapply tctx_incl_tail. eapply (logic_fn_ghost_tctx_incl' [_] _ +[]). apply uniq_curr_logic_fn.
+    eapply tctx_incl_trans. apply tctx_incl_swap. eapply (logic_fn_ghost_tctx_incl' [_; _] _ +[_]).
+    apply find_logic. intros ??(?&?&->&?). eexists _, _. done. eapply tctx_incl_trans. eapply tctx_incl_swap.
+    eapply ghost_update; [done|solve_typing|]. 
+    eapply tctx_incl_trans. eapply (tctx_incl_frame_r +[_; _]). eapply seq_remove. done. eapply tctx_incl_tail. eapply tctx_incl_trans. eapply tctx_incl_swap. eapply permdata_to_box. 
+    iApply type_jump; [solve_typing|solve_extract|solve_typing].
+    rewrite /trans_upper /trans_tail. move=>post [[tc tf][l' []]] [v [lookup Impl]]/=.
+    eexists _, _. split. done. destruct (find_idx_delete _ _ _ lookup) as (?&->). split. done. split. done.
+    intros. apply Impl. rewrite H0 H. done.
   Qed.
     
 End ghostptrtoken_insertremove.
